start to update proofs

shiftreset/Hoare.v
@@ -376,12 +376,7 @@ Module HistoryTriplesValues.
   Proof.
     unfold entails, Proper, respectful, impl, hist_triple, flip.
     intros. subst.
-    apply H1.
-    applys H2.
-    apply H.
-    exact H3.
-    exact H4.
-    exact H5.
+    jauto.
   Qed.
 
   #[global]
@@ -392,11 +387,8 @@ Module HistoryTriplesValues.
     unfold entails, Proper, respectful, impl, hist_triple, flip.
     intros. subst.
     apply H1.
-    applys H2.
-    apply H.
-    exact H3.
-    exact H4.
-    exact H5.
+    specializes H2 H4 H5.
+    apply* H.
   Qed.
 
   (** Structural rules *)
@@ -631,7 +623,7 @@ Module HistoryTriples.
 
   Import SpecAssertions.
 
-  Definition res_compat (pres:eresult) (res:result) :=
+  Definition res_compatible (pres:eresult) (res:result) :=
     match pres, res with
     | enorm v1, norm v2 => v1 = v2
     | eshft (vfun x1 eb) (vfun x2 ek),
@@ -640,37 +632,39 @@ Module HistoryTriples.
         exists r, spec_assert (subst x2 v1 ek) (fk r)
     | _, _ => False
     end.
-  
-  (* < 1 + shift k. k 1 > *)
-  Definition e1p := eshft
-    (vfun "k" (papp (pvar "k") (pval (vint 1))))
-    (vfun "x" (pvar "x")).
 
-  Definition e1s vk := shft
-    "k" (∃ r, unk "k" (vint 1) (r))
-    vk (fun r => rs (ens (fun r1 => \[vk = r1])) r).
+  Module Test.
+    (* < 1 + shift k. k 1 > *)
+    Definition e1p := eshft
+      (vfun "k" (papp (pvar "k") (pval (vint 1))))
+      (vfun "x" (pvar "x")).
 
-  Example e1_compat: forall v,
-    res_compat e1p (e1s v).
-  Proof.
-    unfold e1p, e1s. simpl. intros.
-    unfold spec_assert, pair_valid_under.
-    split; intros.
-    { inverts H0 as H0.
-      apply s_fex. exists v0.
-      remember (Fmap.read p1 "k") as u eqn:H1. symmetry in H1.
-      unfold env_compatible in H. specializes H H1. destr H.
-      specializes H3 v0. unfold pair_valid_under in H3.
-      specializes H3 H0.
-      applys s_unk H.
-      assumption. }
-    { exs. intros.
-      inverts H0 as H0.
-      apply s_rs_val.
-      apply ens_pure_intro.
-      reflexivity.
-    }
-  Qed.
+    Definition e1s vk := shft
+      "k" (∃ r, unk "k" (vint 1) (r))
+      vk (fun r => rs (ens (fun r1 => \[vk = r1])) r).
+
+    Example e1_compat: forall v,
+      res_compatible e1p (e1s v).
+    Proof.
+      unfold e1p, e1s. simpl. intros.
+      unfold spec_assert, pair_valid_under.
+      split; intros.
+      { inverts H0 as H0.
+        apply s_fex. exists v0.
+        remember (Fmap.read p1 "k") as u eqn:H1. symmetry in H1.
+        unfold env_compatible in H. specializes H H1. destr H.
+        specializes H3 v0. unfold pair_valid_under in H3.
+        specializes H3 H0.
+        applys s_unk H.
+        assumption. }
+      { exs. intros.
+        inverts H0 as H0.
+        apply s_rs_val.
+        apply ens_pure_intro.
+        reflexivity.
+      }
+    Qed.
+  End Test.
 
   (** * History triples *)
   (** A #<i>history triple</i># (i.e. not just a "triple", which typically refers to a Hoare triple) also constrains the history of a program. *)
@@ -680,11 +674,12 @@ Module HistoryTriples.
       └───────────[f]──────────┘
   *)
   Definition hist_triple fh e f :=
-    forall p1 s0 s1 h0 h1 h2 v R,
-      satisfies s0 s1 h0 h1 R fh ->
+    forall p1 s0 s1 h0 h1 h2 R0 R Re,
+      satisfies s0 s1 h0 h1 R0 fh ->
       env_compatible p1 s1 ->
-      bigstep p1 h1 e h2 R1 ->
-      satisfies s0 s1 h0 h2 R2 f.
+      res_compatible Re R ->
+      bigstep p1 h1 e h2 Re ->
+      satisfies s0 s1 h0 h2 R f.
 
   (** History triples are contravariant in the history. *)
   #[global]
@@ -695,11 +690,8 @@ Module HistoryTriples.
     unfold entails, Proper, respectful, impl, hist_triple, flip.
     intros. subst.
     apply H1.
-    applys H2.
-    apply H.
-    exact H3.
-    exact H4.
-    exact H5.
+    specializes H H3.
+    specializes H2 H H4 H5.
   Qed.
 
   #[global]
@@ -710,11 +702,8 @@ Module HistoryTriples.
     unfold entails, Proper, respectful, impl, hist_triple, flip.
     intros. subst.
     apply H1.
-    applys H2.
-    apply H.
-    exact H3.
-    exact H4.
-    exact H5.
+    specializes H2 H4 H5.
+    apply* H.
   Qed.
 
   (** Structural rules *)
